Rework Commandline module in basis
CF proofs updated.

For #347

basis/CommandlineProofScript.sml
@@ -6,7 +6,7 @@ val _ = new_theory"CommandlineProof";
 val _ = translation_extends"CommandlineProg";
 
 val wfcl_def = Define`
-  wfcl cl ⇔ EVERY validArg cl ∧ ¬NULL cl ∧ SUM (MAP LENGTH cl) + LENGTH cl <= 256`;
+  wfcl cl <=> EVERY validArg cl ∧ LENGTH cl < 256 * 256 /\ cl <> []`;
 
 val COMMANDLINE_def = Define `
   COMMANDLINE cl =
@@ -17,7 +17,8 @@ val set_thm =
   |> SIMP_RULE(srw_ss())[
        cfHeapsBaseTheory.IOx_def,cl_ffi_part_def,
        cfHeapsBaseTheory.IO_def, set_sepTheory.one_def ]
-  |> SIMP_RULE(srw_ss())[Once FUN_EQ_THM,set_sepTheory.SEP_EXISTS_THM,set_sepTheory.cond_STAR,PULL_EXISTS]
+  |> SIMP_RULE(srw_ss())[Once FUN_EQ_THM,
+        set_sepTheory.SEP_EXISTS_THM,set_sepTheory.cond_STAR,PULL_EXISTS]
   |> Q.SPEC`cl`
 val set_tm = set_thm |> concl |> find_term(pred_setSyntax.is_insert)
 
@@ -39,76 +40,182 @@ val eq_num_v_thm = MATCH_MP (DISCH_ALL eq_v_thm) (EqualityType_NUM_BOOL |> CONJU
 
 val st = get_ml_prog_state();
 
-val Commandline_cline_spec = Q.store_thm("Commandline_cline_spec",
-  `UNIT_TYPE u uv ==>
-    app (p:'ffi ffi_proj) ^(fetch_v "Commandline.cline" st) [uv]
-    (COMMANDLINE cl)
-    (POSTv clinev. & LIST_TYPE STRING_TYPE (MAP implode  cl) clinev * COMMANDLINE cl)`,
-  xcf "Commandline.cline" st
-  \\ xlet_auto >- xsimpl
-  \\ xlet_auto >- xsimpl
-  \\ rename1`W8ARRAY cs`
-  \\ qabbrev_tac`l = MAP ((n2w:num -> word8) o ORD) (FLAT (MAP (\s. s ++ [CHR 0]) cl))`
-  \\ fs [COMMANDLINE_def]
-  \\ xpull
-  \\ `LENGTH l = LENGTH cl + SUM (MAP LENGTH cl)`
-  by (
-    simp[Abbr`l`,LENGTH_FLAT,MAP_MAP_o,o_DEF,SUM_MAP_PLUS,
-         MAP_K_REPLICATE |> SIMP_RULE std_ss [K_DEF],
-         SUM_REPLICATE])
-  \\ `LENGTH l ≤ 256` by fs[wfcl_def]
-  \\ xlet `POSTv u. W8ARRAY cs (l ++ DROP (LENGTH l) (REPLICATE 256 (n2w 0))) * COMMANDLINE cl`
-  >- (
-    xffi
-    \\ fs[COMMANDLINE_def,cfHeapsBaseTheory.IOx_def,cl_ffi_part_def]
+val Commandline_read16bit_spec = Q.store_thm("Commandline_read16bit",
+  `2 <= LENGTH a ==>
+   app (p:'ffi ffi_proj) ^(fetch_v "Commandline.read16bit" st) [av]
+     (W8ARRAY av a)
+     (POSTv v. W8ARRAY av a * & NUM (w2n (EL 0 a) + 256 * w2n (EL 1 a)) v)`,
+  xcf "Commandline.read16bit" st
+  \\ xlet_auto THEN1 xsimpl
+  \\ xlet_auto THEN1 (fs [] \\ xsimpl)
+  \\ xlet_auto THEN1 (fs [] \\ xsimpl)
+  \\ xlet_auto THEN1 (fs [] \\ xsimpl)
+  \\ xlet_auto THEN1 (fs [] \\ xsimpl)
+  \\ xapp \\ xsimpl
+  \\ Cases_on `a` \\ fs [] \\ Cases_on `t` \\ fs [NUM_def]
+  \\ rpt (asm_exists_tac \\ fs [])
+  \\ Cases_on `h` \\ Cases_on `h'` \\ fs []
+  \\ fs [INT_def] \\ intLib.COOPER_TAC);
+
+val Commandline_write16bit_spec = Q.store_thm("Commandline_write16bit",
+  `NUM n nv /\ 2 <= LENGTH a ==>
+   app (p:'ffi ffi_proj) ^(fetch_v "Commandline.write16bit" st) [av;nv]
+     (W8ARRAY av a)
+     (POSTv v. W8ARRAY av (n2w n::n2w (n DIV 256)::TL (TL a)))`,
+  xcf "Commandline.write16bit" st
+  \\ xlet_auto THEN1 xsimpl
+  \\ xlet_auto THEN1 (fs [] \\ xsimpl)
+  \\ xlet_auto THEN1 (fs [] \\ xsimpl)
+  \\ xlet_auto THEN1 (fs [] \\ xsimpl)
+  \\ xapp \\ xsimpl
+  \\ Cases_on `a` \\ fs [] \\ Cases_on `t` \\ fs [NUM_def]
+  \\ rpt (asm_exists_tac \\ fs [])
+  \\ EVAL_TAC);
+
+val SUC_SUC_LENGTH = prove(
+  ``SUC (SUC (LENGTH (TL (TL (REPLICATE (MAX 2 n) x))))) = (MAX 2 n)``,
+  Cases_on `n` \\ fs [] THEN1 EVAL_TAC
+  \\ Cases_on `n'` \\ fs [] THEN1 EVAL_TAC
+  \\ fs [ADD1] \\ rw [MAX_DEF]
+  \\ fs [EVAL ``REPLICATE 2 x``]
+  \\ once_rewrite_tac [ADD_COMM]
+  \\ rewrite_tac [GSYM REPLICATE_APPEND]
+  \\ fs [EVAL ``REPLICATE 2 x``]);
+
+val two_byte_sum = prove(
+  ``k < 65536 ==> k MOD 256 + 256 * (k DIV 256) MOD 256 = k``,
+  rw []
+  \\ `(k DIV 256) MOD 256 = k DIV 256` by
+        (match_mp_tac LESS_MOD \\ fs [DIV_LT_X,wfcl_def]) \\ fs []
+  \\ `(k DIV 256) * 256 + k MOD 256 = k` by metis_tac [DIVISION,EVAL ``0 < 256n``]
+  \\ fs []);
+
+val LESS_LENGTH_EXISTS = prove(
+  ``!xs n. n < LENGTH xs ==> ?ys y ts. xs = ys ++ y::ts /\ LENGTH ys = n``,
+  Induct \\ fs [] \\ Cases_on `n` \\ fs []
+  \\ rw [] \\ res_tac \\ fs [] \\ rveq \\ fs []
+  \\ qexists_tac `h::ys` \\ fs []);
+
+val DROP_SUC_LENGTH_MAP = prove(
+  ``(DROP (SUC (LENGTH ys)) (MAP f ys ⧺ y::ts)) = ts``,
+  qsuff_tac `MAP f ys ⧺ y::ts = (MAP f ys ⧺ [y]) ++ ts /\
+             SUC (LENGTH ys) = LENGTH (MAP f ys ⧺ [y])`
+  THEN1 simp_tac std_ss [DROP_LENGTH_APPEND] \\ fs []);
+
+val Commandline_cloop_spec = Q.store_thm("Commandline_cloop_spec",
+  `!n nv av cv a.
+     LIST_TYPE STRING_TYPE (DROP n (MAP implode cl)) cv /\
+     NUM n nv /\ n <= LENGTH cl /\ LENGTH a = 2 ==>
+     app (p:'ffi ffi_proj) ^(fetch_v "Commandline.cloop" st) [av; nv; cv]
+      (COMMANDLINE cl * W8ARRAY av a)
+      (POSTv v. & LIST_TYPE STRING_TYPE (MAP implode cl) v * COMMANDLINE cl)`,
+  Induct \\ rw []
+  THEN1
+   (xcf "Commandline.cloop" st
+    \\ xlet_auto THEN1 xsimpl
+    \\ xif \\ asm_exists_tac \\ fs []
+    \\ xvar \\ xsimpl)
+  \\ xcf "Commandline.cloop" st
+  \\ xlet_auto THEN1 xsimpl
+  \\ xif \\ asm_exists_tac \\ fs []
+  \\ rpt (xlet_auto THEN1 xsimpl)
+  \\ fs [ADD1,intLib.COOPER_PROVE ``& (n+1) - 1 = (& n):int``,GSYM NUM_def]
+  \\ qabbrev_tac `x = EL n cl`
+  \\ fs [COMMANDLINE_def] \\ xpull
+  \\ `(n DIV 256) * 256 + n MOD 256 = n` by metis_tac [DIVISION,EVAL ``0 < 256n``]
+  \\ `(n DIV 256) MOD 256 = n DIV 256` by
+        (match_mp_tac LESS_MOD \\ fs [DIV_LT_X,wfcl_def])
+  \\ xlet `POSTv v.
+       W8ARRAY av (n2w (LENGTH x)::n2w (LENGTH x DIV 256)::[]) * COMMANDLINE cl`
+  THEN1
+   (xffi
+    \\ fs[cfHeapsBaseTheory.IOx_def,cl_ffi_part_def,COMMANDLINE_def]
     \\ xsimpl
     \\ qmatch_goalsub_abbrev_tac`IO s u ns`
     \\ map_every qexists_tac [`emp`, `s`, `s`, `u`, `ns`]
     \\ xsimpl
-    \\ fs[Abbr`u`,Abbr`ns`,cfHeapsBaseTheory.mk_ffi_next_def,ffi_getArgs_def,GSYM cfHeapsBaseTheory.encode_list_def,Abbr`s`]
-    \\ simp[EVERY_MAP, LENGTH_REPLICATE, Abbr`l`]
-    \\ rw[encode_def] \\ fs[EVERY_REPLICATE])
-  \\ xfun_spec`foo``∀c cv. CHAR c cv ⇒ app p foo [cv] emp (POSTv v. &(BOOL (CHR 0 = c) v))`
-  >- (
-    rw[]
-    \\ xapp
-    \\ xlet_auto >- xsimpl
-    \\ xapp_spec eq_num_v_thm
-    \\ instantiate
+    \\ unabbrev_all_tac \\ fs []
+    \\ fs[cfHeapsBaseTheory.mk_ffi_next_def,ffi_get_arg_length_def,
+           GSYM cfHeapsBaseTheory.encode_list_def,LENGTH_EQ_NUM_compute]
+    \\ fs [wfcl_def])
+  \\ rpt (xlet_auto THEN1 xsimpl)
+  \\ qmatch_goalsub_abbrev_tac`W8ARRAY av1 bytes`
+  \\ `LENGTH x < 65536` by
+       (fs [wfcl_def,SUC_SUC_LENGTH,Abbr`x`] \\ `n < LENGTH cl` by fs []
+        \\ fs [EVERY_EL] \\ first_x_assum drule \\ fs [validArg_def])
+  \\ xlet `POSTv v. W8ARRAY av1 (MAP (n2w o ORD) x ++ DROP (LENGTH x) bytes) *
+       W8ARRAY av [n2w (STRLEN x); n2w (STRLEN x DIV 256)] * COMMANDLINE cl`
+  THEN1 (xffi
+    \\ fs[cfHeapsBaseTheory.IOx_def,cl_ffi_part_def,COMMANDLINE_def]
+    \\ qabbrev_tac `extra = W8ARRAY av [n2w (STRLEN x); n2w (STRLEN x DIV 256)]`
     \\ xsimpl
-    \\ simp[CHAR_EQ_THM,BOOL_def] )
-  \\ xlet_auto >- xsimpl
+    \\ qmatch_goalsub_abbrev_tac`IO s u ns`
+    \\ map_every qexists_tac [`extra`, `s`, `s`, `u`, `ns`]
+    \\ xsimpl
+    \\ unabbrev_all_tac \\ fs []
+    \\ fs[cfHeapsBaseTheory.mk_ffi_next_def,ffi_get_arg_def,
+           GSYM cfHeapsBaseTheory.encode_list_def,LENGTH_EQ_NUM_compute]
+    \\ fs [wfcl_def,SUC_SUC_LENGTH,two_byte_sum])
+  \\ xlet_auto
+  THEN1 (xsimpl \\ fs [SUC_SUC_LENGTH,two_byte_sum])
+  \\ xlet_auto THEN1 (xcon \\ xsimpl)
   \\ xapp
-  \\ fs[COMMANDLINE_def]
-  \\ instantiate
+  \\ fs [COMMANDLINE_def] \\ xsimpl
+  \\ fs [LENGTH_EQ_NUM_compute]
+  \\ rveq \\ fs []
+  \\ fs [GSYM LESS_EQ,GSYM ADD1]
+  \\ drule LESS_LENGTH_EXISTS
+  \\ strip_tac \\ rw [] \\ fs []
+  \\ `LENGTH ys = LENGTH (MAP implode ys)` by fs []
+  \\ asm_rewrite_tac [DROP_LENGTH_APPEND]
+  \\ fs [LIST_TYPE_def,DROP_SUC_LENGTH_MAP]
+  \\ fs [two_byte_sum]
+  \\ rfs [two_byte_sum]
+  \\ fs [mlstringTheory.implode_def]
+  \\ qpat_x_assum `_ sv` mp_tac
+  \\ `LENGTH x = LENGTH (MAP ((n2w:num->word8) ∘ ORD) x)` by fs []
+  \\ asm_rewrite_tac [TAKE_LENGTH_APPEND]
+  \\ full_simp_tac std_ss [GSYM APPEND_ASSOC,APPEND,EL_LENGTH_APPEND,NULL,HD]
+  \\ fs [MAP_MAP_o]
+  \\ qmatch_goalsub_abbrev_tac `MAP ff`
+  \\ qsuff_tac `!xs. MAP ff xs = xs` THEN1 fs []
+  \\ Induct \\ fs [Abbr `ff`] \\ fs [ORD_BOUND,CHR_ORD]);
+
+val Commandline_cline_spec = Q.store_thm("Commandline_cline_spec",
+  `UNIT_TYPE u uv ==>
+   app (p:'ffi ffi_proj) ^(fetch_v "Commandline.cline" st) [uv]
+    (COMMANDLINE cl)
+    (POSTv v. & LIST_TYPE STRING_TYPE (MAP implode cl) v * COMMANDLINE cl)`,
+  xcf "Commandline.cline" st
+  \\ xlet_auto >- xsimpl
+  \\ xlet_auto >- xsimpl
+  \\ qmatch_goalsub_rename_tac `W8ARRAY av`
+  \\ fs [EVAL ``REPLICATE 2 x``]
+  \\ fs [COMMANDLINE_def]
+  \\ xpull
+  \\ xlet `POSTv v.
+       (W8ARRAY av [n2w (LENGTH cl); n2w (LENGTH cl DIV 256)] * IOx cl_ffi_part cl)`
+  THEN1
+   (xffi
+    \\ fs[cfHeapsBaseTheory.IOx_def,cl_ffi_part_def]
+    \\ xsimpl
+    \\ qmatch_goalsub_abbrev_tac`IO s u ns`
+    \\ map_every qexists_tac [`emp`, `s`, `s`, `u`, `ns`]
+    \\ xsimpl
+    \\ unabbrev_all_tac \\ fs []
+    \\ fs[cfHeapsBaseTheory.mk_ffi_next_def,ffi_get_arg_count_def,
+           GSYM cfHeapsBaseTheory.encode_list_def]
+    \\ fs [wfcl_def])
+  \\ xlet_auto >- xsimpl
+  \\ xlet_auto THEN1 (xcon \\ xsimpl)
+  \\ xapp
+  \\ fs [COMMANDLINE_def]
   \\ xsimpl
-  \\ qexists_tac`(=) (CHR 0)`
-  \\ conj_tac
-  >- (
-    Q.ISPEC_THEN`p`match_mp_tac (Q.GEN`p` app_basic_IMP_Arrow)
-    \\ fs[app_def] )
-  \\ fs[wfcl_def]
-  \\ simp[TAKE_APPEND,TAKE_LENGTH_TOO_LONG,Abbr`l`,mlstringTheory.TOKENS_eq_tokens_sym,
-          MAP_TAKE,MAP_MAP_o,CHR_w2n_n2w_ORD,MAP_DROP,map_replicate,DROP_REPLICATE]
-  \\ fsrw_tac[ETA_ss][GSYM SNOC_APPEND]
-  \\ Q.ISPEC_THEN`cl`FULL_STRUCT_CASES_TAC SNOC_CASES >- fs[]
-  \\ simp[MAP_SNOC,FLAT_SNOC]
-  \\ qmatch_goalsub_abbrev_tac`l1 ++ SNOC nl x ++ REPLICATE _ _`
-  \\ qmatch_goalsub_abbrev_tac`l1 ++ SNOC nl x ++ l3`
-  \\ `l1 ++ SNOC nl x ++ l3 = (l1 ++ x) ++ nl::l3` by simp[SNOC_APPEND]
-  \\ pop_assum SUBST_ALL_TAC
-  \\ simp[TOKENS_APPEND,Abbr`nl`]
-  \\ simp[Abbr`l3`,(TOKENS_NIL|>SPEC_ALL|>EQ_IMP_RULE |> #2),EVERY_REPLICATE]
-  \\ qmatch_goalsub_abbrev_tac`((=) nl)`
-  \\ `l1 ++ x = FRONT (FLAT (MAP (SNOC nl) (SNOC x l)))`
-  by ( simp[Abbr`l1`,FRONT_APPEND] )
-  \\ simp[]
-  \\ DEP_REWRITE_TAC[TOKENS_FRONT]
-  \\ simp[FLAT_EQ_NIL,NULL_EQ,EXISTS_MAP,LAST_FLAT]
-  \\ DEP_REWRITE_TAC[FILTER_EQ_ID |> SPEC_ALL |> EQ_IMP_RULE |> #2]
-  \\ simp[EVERY_MAP,NULL_EQ]
-  \\ DEP_REWRITE_TAC[TOKENS_FLAT_MAP_SNOC]
-  \\ fs[EVERY_SNOC,validArg_def,EVERY_MEM,NULL_EQ,MAP_SNOC]);
+  \\ `LENGTH cl <= LENGTH cl` by fs []
+  \\ asm_exists_tac \\ fs [] \\ xsimpl
+  \\ `DROP (LENGTH cl) (MAP implode cl) = []` by fs [DROP_NIL]
+  \\ fs [LIST_TYPE_def]
+  \\ fs [wfcl_def] \\ rfs [two_byte_sum]);
 
 val hd_v_thm = fetch "ListProg" "hd_v_thm";
 val mlstring_hd_v_thm = hd_v_thm |> INST_TYPE [alpha |-> mlstringSyntax.mlstring_ty]
@@ -118,15 +225,14 @@ val Commandline_name_spec = Q.store_thm("Commandline_name_spec",
     app (p:'ffi ffi_proj) ^(fetch_v "Commandline.name" st) [uv]
     (COMMANDLINE cl)
     (POSTv namev. & STRING_TYPE (implode (HD cl)) namev * COMMANDLINE cl)`,
-    xcf "Commandline.name" st
-    \\ xlet `POSTv vz. & UNIT_TYPE () vz * COMMANDLINE cl`
-    >-(xcon \\ xsimpl)
-    \\ xlet `POSTv cs. & LIST_TYPE STRING_TYPE (MAP implode cl) cs * COMMANDLINE cl`
-    >-(xapp \\ rw[])
-    \\ Cases_on`cl=[]` >- ( fs[COMMANDLINE_def] \\ xpull \\ fs[wfcl_def] )
-    \\ xapp_spec mlstring_hd_v_thm
-    \\ xsimpl \\ instantiate \\ Cases_on `cl` \\ rw[]
-);
+  xcf "Commandline.name" st
+  \\ xlet `POSTv vz. & UNIT_TYPE () vz * COMMANDLINE cl`
+  >-(xcon \\ xsimpl)
+  \\ xlet `POSTv cs. & LIST_TYPE STRING_TYPE (MAP implode cl) cs * COMMANDLINE cl`
+  >-(xapp \\ rw[])
+  \\ Cases_on`cl=[]` >- ( fs[COMMANDLINE_def] \\ xpull \\ fs[wfcl_def] )
+  \\ xapp_spec mlstring_hd_v_thm
+  \\ xsimpl \\ instantiate \\ Cases_on `cl` \\ rw[]);
 
 val tl_v_thm = fetch "ListProg" "tl_v_thm";
 val mlstring_tl_v_thm = tl_v_thm |> INST_TYPE [alpha |-> mlstringSyntax.mlstring_ty]
@@ -135,36 +241,38 @@ val Commandline_arguments_spec = Q.store_thm("Commandline_arguments_spec",
   `UNIT_TYPE u uv ==>
     app (p:'ffi ffi_proj) ^(fetch_v "Commandline.arguments" st) [uv]
     (COMMANDLINE cl)
-    (POSTv argv. & LIST_TYPE STRING_TYPE (TL (MAP implode cl)) argv * COMMANDLINE cl)`,
-    xcf "Commandline.arguments" st
-    \\ xlet `POSTv vz. & UNIT_TYPE () vz * COMMANDLINE cl`
-    >-(xcon \\ xsimpl)
-    \\ xlet `POSTv cs. & LIST_TYPE STRING_TYPE (MAP implode cl) cs * COMMANDLINE cl`
-    >-(xapp \\ rw[])
-    \\ Cases_on`cl=[]` >- ( fs[COMMANDLINE_def] \\ xpull \\ fs[wfcl_def] )
-    \\ xapp_spec mlstring_tl_v_thm \\ xsimpl \\ instantiate \\ Cases_on `cl` \\ rw[mllistTheory.tl_def]
-);
+    (POSTv argv. & LIST_TYPE STRING_TYPE
+       (TL (MAP implode cl)) argv * COMMANDLINE cl)`,
+  xcf "Commandline.arguments" st
+  \\ xlet `POSTv vz. & UNIT_TYPE () vz * COMMANDLINE cl`
+  >-(xcon \\ xsimpl)
+  \\ xlet `POSTv cs. & LIST_TYPE STRING_TYPE (MAP implode cl) cs * COMMANDLINE cl`
+  >-(xapp \\ rw[])
+  \\ Cases_on`cl=[]` >- ( fs[COMMANDLINE_def] \\ xpull \\ fs[wfcl_def] )
+  \\ xapp_spec mlstring_tl_v_thm \\ xsimpl \\ instantiate
+  \\ Cases_on `cl` \\ rw[mllistTheory.tl_def]);
 
 fun prove_hprop_inj_tac thm =
     rw[HPROP_INJ_def, GSYM STAR_ASSOC, SEP_CLAUSES, SEP_EXISTS_THM, HCOND_EXTRACT] >>
       EQ_TAC >-(DISCH_TAC >> IMP_RES_TAC thm >> rw[]) >> rw[];
 
 val UNIQUE_COMMANDLINE = Q.store_thm("UNIQUE_COMMANDLINE",
-`!s cl1 cl2 H1 H2. VALID_HEAP s ==>
-(COMMANDLINE cl1 * H1) s /\ (COMMANDLINE cl2 * H2) s ==> cl2 = cl1`,
-rw[COMMANDLINE_def, cfHeapsBaseTheory.IOx_def, cl_ffi_part_def, encode_def, cfHeapsBaseTheory.encode_list_def, GSYM STAR_ASSOC] >>
-IMP_RES_TAC FRAME_UNIQUE_IO >>
-fs[] >> rw[] >>
-sg `!l1 l2. (MAP Str l1 = MAP Str l2) ==> l2 = l1`
->-(
+  `!s cl1 cl2 H1 H2. VALID_HEAP s ==>
+     (COMMANDLINE cl1 * H1) s /\ (COMMANDLINE cl2 * H2) s ==> cl2 = cl1`,
+  rw[COMMANDLINE_def, cfHeapsBaseTheory.IOx_def, cl_ffi_part_def,
+     encode_def, cfHeapsBaseTheory.encode_list_def, GSYM STAR_ASSOC] >>
+  IMP_RES_TAC FRAME_UNIQUE_IO >>
+  fs[] >> rw[] >>
+  sg `!l1 l2. (MAP Str l1 = MAP Str l2) ==> l2 = l1`
+  >-(
     Induct_on `l2` >-(rw[])>>
     rw[] >> fs[] >>
     Cases_on `l1` >-(fs[])>>  fs[]
-) >>
-fs[]);
+  ) >>
+  fs[]);
 
 val COMMANDLINE_HPROP_INJ = Q.store_thm("COMMANDLINE_HPROP_INJ[hprop_inj]",
-`!cl1 cl2. HPROP_INJ (COMMANDLINE cl1) (COMMANDLINE cl2) (cl2 = cl1)`,
-prove_hprop_inj_tac UNIQUE_COMMANDLINE);
+  `!cl1 cl2. HPROP_INJ (COMMANDLINE cl1) (COMMANDLINE cl2) (cl2 = cl1)`,
+  prove_hprop_inj_tac UNIQUE_COMMANDLINE);
 
 val _ = export_theory();
