basis/TextIOProofScript.sml
@@ -854,7 +854,7 @@ val output_spec = Q.store_thm("output_spec",
   fs[insert_atI_def] >>
   xlet_auto >- xsimpl >>
   xlet_auto >- xsimpl >>
-  xlet`POSTv mv. &NUM (MIN (strlen s) 255) mv * IOx fs_ffi_part fs * W8ARRAY (Loc 1) (h1::h2::h3::rest)`
+  xlet`POSTv mv. &NUM (MIN (strlen s) 255) mv * IOx fs_ffi_part fs * W8ARRAY (Loc 0) (h1::h2::h3::rest)`
   >- (
     xif
     >- (xret \\ xsimpl \\ fs[NUM_def,INT_def,MIN_DEF] )
@@ -932,7 +932,7 @@ val read_spec = Q.store_thm("read_spec",
    NTAC 2 (xlet_auto >- (fs[LUPDATE_def] >> xsimpl)) >>
    simp[LUPDATE_def,EVAL ``LUPDATE rr 1 (zz :: tt)``] >>
    cases_on`get_file_content fs fd`
-   >-(xlet`POSTv v. W8ARRAY (Loc 1) (1w::n::h3::rest) * IOx fs_ffi_part fs`
+   >-(xlet`POSTv v. W8ARRAY (Loc 0) (1w::n::h3::rest) * IOx fs_ffi_part fs`
       >-(xffi >> xsimpl >>
          fs[iobuff_loc,IOFS_def,IOx_def,fs_ffi_part_def, mk_ffi_next_def] >>
          qmatch_goalsub_abbrev_tac`IO st f ns` >>
@@ -1120,7 +1120,7 @@ val input_IOFS_spec = Q.store_thm("input_IOFS_spec",
   Induct_on`N` >> rw[]
   >-(xapp >> fs[IOFS_def,IOFS_iobuff_def] >> xpull >>
      NTAC 2 (xlet_auto >- xsimpl) >>
-     rename [`W8ARRAY (Loc 1) bdef`] >>
+     rename [`W8ARRAY (Loc 0) bdef`] >>
      Cases_on `bdef` >> fs[] >> qmatch_goalsub_abbrev_tac`h1 :: t` >>
      Cases_on `t` >> fs[] >> qmatch_goalsub_abbrev_tac`h1 :: h2 :: t'` >>
      Cases_on `t'` >> fs[] >> qmatch_goalsub_abbrev_tac`h1 :: h2 :: h3 :: rest` >>
@@ -1143,7 +1143,7 @@ val input_IOFS_spec = Q.store_thm("input_IOFS_spec",
   rw[] >> cases_on`len'`
   >-(rw[] >>
      NTAC 2 (xlet_auto >- xsimpl) >>
-     rename [`W8ARRAY (Loc 1) bdef`] >>
+     rename [`W8ARRAY (Loc 0) bdef`] >>
      Cases_on `bdef` >> fs[] >> qmatch_goalsub_abbrev_tac`h1 :: t` >>
      Cases_on `t` >> fs[] >> qmatch_goalsub_abbrev_tac`h1 :: h2 :: t'` >>
      Cases_on `t'` >> fs[] >> qmatch_goalsub_abbrev_tac`h1 :: h2 :: h3 :: rest` >>
@@ -1161,7 +1161,7 @@ val input_IOFS_spec = Q.store_thm("input_IOFS_spec",
      `fs1 = fs2` suffices_by xsimpl >>
      unabbrev_all_tac >> fs[IO_fs_component_equality,ALIST_FUPDKEY_unchanged]) >>
   NTAC 2 (xlet_auto >- xsimpl) >>
-  rename [`W8ARRAY (Loc 1) bdef`] >>
+  rename [`W8ARRAY (Loc 0) bdef`] >>
   Cases_on `bdef` >> fs[] >> qmatch_goalsub_abbrev_tac`h1 :: t` >>
   Cases_on `t` >> fs[] >> qmatch_goalsub_abbrev_tac`h1 :: h2 :: t'` >>
   Cases_on `t'` >> fs[] >> qmatch_goalsub_abbrev_tac`h1 :: h2 :: h3 :: rest` >>
